\documentclass{article}
\usepackage{amsmath}
\usepackage{amsthm}
\usepackage{amssymb}
\usepackage{enumerate}
\usepackage{graphicx}

\begin{document}
    \title{MA 4\_4 Exercise}
    \author{Wang Yue from CS Elite Class}
    \date{\today}

    \maketitle

    \subsection*{32. $\lim_{x \to 0}\frac{\cos mx - \cos nx}{x^2}$}

    $$\begin{aligned}
        \lim_{x \to 0}\frac{\cos mx - \cos nx}{x^2} &= \lim_{x \to 0} \frac{(1 - \frac 1 2 (mx)^2) - (1 - \frac 1 2 (nx)^2)}{x^2} \\
        &= \lim_{x \to 0}\frac{\frac 1 2(n^2 - m^2)x^2}{x^2} \\
        &= \lim_{x \to 0}\frac{n^2 - m^2}{2}
    \end{aligned}$$

    \subsection*{39. $\lim_{x \to 0}\frac{\cos x - 1 + \frac 1 2 x^2}{x^4}$}

    $$\begin{aligned}
        \lim_{x \to 0}\frac{\cos x - 1 + \frac 1 2 x^2}{x^4} &= \lim_{x \to 0}\frac{1 - \frac 1 2 x^2 + \frac{1}{24} x^4 - 1 + \frac 1 2 x^2}{x^4} \\
        &= \lim_{x \to 0}\frac{\frac{1}{24} x^4}{x^4} \\
        &= \frac{1}{24}
    \end{aligned}$$

    \subsection*{38. $\lim_{x \to 0}\frac{e^x - e^{-x} - 2x}{x - \sin x}$}

    $$\begin{aligned}
        \lim_{x \to 0}\frac{e^x - e^{-x} - 2x}{x - \sin x} &= \lim_{x \to 0}\frac{(1 + x + \frac 1 2 x^2 + \frac 1 6 x^3) - (1 - x + \frac 1 2 x^2 - \frac 1 6 x^3) - 2x}{x - (x - \frac{1}{6}x^3)} \\
        &= \frac{2x + \frac 1 3 x^3 - 2x}{\frac 1 6 x^3} \\
        &= 2
    \end{aligned}$$

    % 32 39 38

    \subsection*{$\lim_{x \to 0}\frac{e^{x^3} - 1 - x^3}{(\sin 2x)^6}$}

    $$\begin{aligned}
        \lim_{x \to 0}\frac{e^{x^3} - 1 - x^3}{(\sin 2x)^6} &= \lim_{x \to 0}\frac{1 + x^3 + \frac 1 2 x^6 - 1 - x^3}{(2x)^6} \\
        &= \lim_{x \to 0}\frac{\frac{x^6}{2}}{2^6 x^6} \\
        &= \frac{1}{128}
    \end{aligned}$$

    \subsection*{$\lim_{x \to \infty}(x + \frac 1 2)\ln(1 + \frac 1 x)$}

    $$\begin{aligned}
        \lim_{x \to \infty}(x + \frac 1 2)\ln(1 + \frac 1 x) &= \lim_{x \to \infty}(x + \frac 1 2)(\frac 1 x - \frac{1}{2x^2}) \\
        &= \lim_{x \to \infty}(1 - \frac{1}{2x} + \frac{1}{2x} - \frac{1}{4x^2}) \\
        &= \lim_{x \to \infty}(1 - \frac{1}{4x^2}) \\
        &= 1
    \end{aligned}$$

    \subsection*{$\lim_{x \to 0}(\frac 1 x - \frac{1}{e^x - 1})$}

    $$\begin{aligned}
        \lim_{x \to 0}(\frac 1 x - \frac{1}{e^x - 1}) &= \lim_{x \to 0}\frac{e^x - 1 - x}{x(e^x - 1)} \\
        &= \lim_{x \to 0}\frac{1 + x + \frac 1 2 x^2 - 1 - x}{x(1 + x + \frac 1 2 x^2 - 1)} \\
        &= \lim_{x \to 0}\frac{1}{2(1 + \frac x 2)} \\
        &= \frac{1}{2}
    \end{aligned}$$

    \subsection*{$\lim_{x \to 0^+}\frac{e^x - 1 - x}{\sqrt{1 - x} - \cos \sqrt x}$}

    $$\begin{aligned}
        \lim_{x \to 0^+}\frac{e^x - 1 - x}{\sqrt{1 - x} - \cos \sqrt{x}} &= \lim_{x \to 0^+}\frac{1 + x + \frac 1 2 x^2 - 1 - x}{1 - \frac 1 2 x - \frac 1 8 x^2 - (1 - \frac 1 2 x)} \\
        &= \lim_{x \to 0^+}\frac{\frac{x^2}{2}}{-\frac{x^2}{8}} \\
        &= -4
    \end{aligned}$$

\end{document}