\documentclass{article}
\usepackage{amsmath}
\usepackage{amsthm}
\usepackage{amssymb}
\usepackage{enumerate}
\usepackage{graphicx}

\begin{document}
    \title{Exercise 7\_1}
    \author{Wang Yue from CS Elite Class}
    \date{\today}
    \maketitle

    \section*{Exercise 7.3}

    \subsection*{39. }

    \begin{enumerate}[(a)]
        \item Use trigonometric substitution to verify that $$\int_0^x \sqrt{a^2 - t^2} dt = \frac 1 2 a^2 \sin^{-1}(x / a) + \frac 1 2 x \sqrt{a^2 - x^2}$$

        \begin{proof}

            Let $t = a\sin \theta$, then $\theta = \arcsin \frac t a, \cos \theta = \frac{\sqrt{a^2 - t^2}}{a}$, so

            $$\begin{aligned}
                \int \sqrt{a^2 - t^2} dt &= \int \sqrt{a^2 - a^2 \sin ^2 \theta} a \cos \theta d \theta \\
                &= \int a^2 \cos ^2 \theta d \theta \\
                &= \int \frac{a^2}{2} + \frac{a^2 \cos 2 \theta}{2} d \theta \\
                &= \frac{a^2}{2} \theta + \frac{a^2}{4} \sin 2\theta + C \\
                &= \frac{a^2}{2} \sin^{-1} \frac{t}{a} \times (2 \frac{t}{a} \frac{\sqrt{a^2 - t^2}}{a}) + C \\
                &= \frac{a^2\sin ^{-1} \frac t a}{2} + \frac{t \sqrt{a^2 - t^2}}{2} + C
            \end{aligned}$$

            $$\therefore \begin{aligned}
                \int_0^x \sqrt{a^2 - t^2} dt &= (\frac{a^2\sin ^{-1} \frac t a}{2} + \frac{t \sqrt{a^2 - t^2}}{2}) \biggl |_0^x \\
                &= \frac{1}{2} a^2 \sin^{-1} \frac x a + \frac 1 2 x \sqrt{a^2 - x^2}
            \end{aligned}$$
        \end{proof}

        \item Use the figure to give trigonometric interpretations of both terms on the right side of the equation in part (a).

        Let the area of the sector be $S_1$ and the area of the triangular be $S_2$.

        By the figure, we have:

        $$\left\{ \begin{array}{ll}
            \theta &= \arcsin \frac{x}{a} \\
            S_{1} &= \frac{1}{2} x \sqrt{a^2 - x^2} \\
            s_{2} &= \frac{1}{2} \theta a^2
        \end{array} \right.$$

        $$\therefore S = S_1 + S_2 = \frac 1 2 a^2 \sin^{-1}(x / a) + \frac 1 2 x \sqrt{a^2 - x^2} = \int_0^x \sqrt{a^2 - t^2} dt$$

    \end{enumerate}

    \section*{Exercise 7.1}

    \subsection*{7. $\int (x^2 + 2x) \cos x dx$}

    $$\begin{aligned}
        \int (x^2 + 2x) \cos x dx &= \int (x^2 + 2x) d\sin x \\
        &= (x^2 + 2x) \sin x - \int \sin x d(x^2 + 2x) \\
        &= (x^2 + 2x) \sin x - \int (2x + 2) \sin x dx \\
        &= (x^2 + 2x) \sin x + \int (2x + 2) d \cos x \\
        &= (x^2 + 2x) \sin x + (2x + 2) \cos x - \int \cos x d(2x + 2) \\
        &= (x^2 + 2x) \sin x + (2x + 2) \cos x - \int 2 \cos x dx \\
        &= (x^2 + 2x - 2) \sin x + (2x + 2) \cos x + C
    \end{aligned}$$

    \subsection*{9. $\int \ln \sqrt[3]{x} dx$}

    $$\begin{aligned}
        \int \ln \sqrt[3]{x} dx &= \frac 1 3 \int \ln x dx \\
        &= \frac 1 3 \times \frac 1 x + C \\
        &= \frac{1}{3x} + C
    \end{aligned}$$

    \subsection*{10. $\int \sin^{-1} x dx $}

    $$\begin{aligned}
        \int \sin^{-1} x dx &= x \sin^{-1}x - \int x d \sin^{-1} x \\
        &= x\arcsin x - \int \frac{x}{\sqrt{1 - x^2}} dx \\
        &= x \arcsin x - \int \frac{dx^2}{2\sqrt{1 - x^2}} \\
        &= x \arcsin x + \sqrt{1 - x^2} + C
    \end{aligned}$$
    
    \subsection*{15. $\int (\ln x)^2 dx$}

    $$\begin{aligned}
        \int (\ln x)^2 dx &= x (\ln x)^2 - \int x d(\ln x)^2 \\
        &= x(\ln x)^2 - \int 2 \ln x dx \\
        &= x(\ln x)^2 - 2(x \ln x - x) + C \\
        &= x(\ln x)^2 - 2x \ln x + 2x + C
    \end{aligned}$$

    \subsection*{17. $\int e^{2\theta} \sin 3\theta d\theta$}

    $$\begin{aligned}
        \int e^{2\theta} \sin 3\theta d\theta &= \frac 1 2 \int \sin 3\theta de^{2\theta} \\
        &= \frac 1 2  (e^{2\theta}\sin 3\theta  - \int e^{2\theta} d \sin 3\theta) \\
        &= \frac 1 2 e^{2\theta} \sin 3\theta - \frac 3 2 \int e^{2\theta}\cos 3\theta d\theta \\
        &= \frac 1 2 e^{2\theta} \sin 3\theta - \frac 3 4 \int \cos 3\theta de^{2\theta} \\
        &= \frac 1 2 e^{2\theta} \sin 3\theta - \frac 3 4 e^{2\theta} \cos 3\theta + \frac 3 4 \int e^{2\theta} d \cos 3\theta \\
        &= \frac 1 2 e^{2\theta} \sin 3\theta - \frac 3 4 e^{2\theta} \cos 3\theta - \frac 9 4 \int e^{2\theta} \sin 3\theta d\theta \\
    \end{aligned}$$

    $$\therefore \int e^{2\theta} \sin 3\theta d\theta = \frac{4}{13}e^{2\theta}(\frac 1 2 \sin 3\theta - \frac 3 4 \cos 3\theta) = e^{2\theta}(\frac{2}{13} \sin 3\theta - \frac{3}{13} \cos 3\theta)$$

    \subsection*{21. $\int \frac{xe^{2x}}{(1 + 2x)^2} dx$}



    \subsection*{26. $\int_4^9 \frac{\ln y}{\sqrt y} dy$}



    $$\begin{aligned}
        \int_4^9 \frac{\ln y}{\sqrt y} dy &= 2\int_4^9 \ln y d\sqrt y \\
        &= 2(\ln y \sqrt y) \biggl |_4^9 - 2 \int_4^9 \sqrt{y} d\ln y \\
        &= 2(6\ln 3 - 4\ln 2) - 2 \int_4^9 \frac{\sqrt{y}}{y} dy \\
        &= 12\ln 3 - 8\ln 2 - 4(\sqrt y) \biggl |_4^9 \\
        &= 12\ln 3 - 8\ln 2 - 4
    \end{aligned}$$

    \subsection*{30. $\int_1^{\sqrt 3} \arctan\frac 1 x dx$}

    Let $u = \frac 1 x, x = \frac 1 u$, then 
    
    $$\begin{aligned}
        \int_1^{\sqrt 3} \arctan \frac 1 x dx &= \int_1^{\frac{\sqrt{3}}{3}} \arctan u d\frac 1 u \\
        &= \int_1^{\frac{\sqrt 3}{3}} -\frac{\arctan u}{u} du \\
        &= -\int_1^{\frac{\sqrt 3}{3}} \frac{1}{u} d \frac{1}{1 + u^2} \\
        &= -(\frac{1}{u(1 + u^2)})\biggl |_1^{\frac{\sqrt 3}{3}} + \int_1^{\frac{\sqrt 3}{3}} \frac{1}{1 + u^2} d\frac 1 u \\
        &= -(\frac{9}{4\sqrt 3} - \frac 1 2) + \int_1^{\sqrt 3} \frac{x^2 + 1 - 1}{x^2 + 1} dx \\
        &= \frac 1 2 - \frac{3\sqrt 3}{4} + \int_1^{\sqrt 3}(1 - \frac{1}{1 + x^2}) dx \\
        &= \frac 1 2 - \frac{3 \sqrt 3}{4} + (x - \arctan x) \biggl |_1^{\sqrt 3} \\
        &= \frac 1 2 - \frac{3\sqrt 3}{4} + \sqrt 3 - \frac \pi 3 - 1 + \frac \pi 4 \\
        &= \frac{\sqrt 3}{4} - \frac{\pi}{12} - \frac 1 2
    \end{aligned}$$

    \subsection*{37. $\int \cos x \sqrt x dx$}

    Let $u = \sqrt x, x = u^2$, then 

    $$\begin{aligned}
        \int \cos \sqrt x dx &= \int 2u \cos u du \\
        &= 2\int u d\sin u \\
        &= 2 u \sin u - 2 \int \sin u du \\
        &= 2 u \sin u + 2 \cos u + C \\
        &= 2 \sqrt x \sin \sqrt x + 2 \cos \sqrt x + C
    \end{aligned}$$

    \subsection*{38. $\int t^3e^{t^2} dt$}

    $$\begin{aligned}
        \int t^3e^{t^2} dt &= \frac 1 2 \int t^2 e^{t^2} d t^2 \\
        &= \frac 1 2(t^2 - 1)e^{t^2} + C
    \end{aligned}$$
    
    \subsection*{70. }

    \begin{enumerate}[(a)]
        \item Use integration by parts to show that $$\int f(x) dx = xf(x) - \int x f'(x) dx$$

        \begin{proof}

            $\because \int f(x) d g(x) = f(x)g(x) - \int g(x) d f(x)$

            $\therefore $ let $g(x) = x$, then $$\int f(x) dx = xf(x) - \int x f'(x) dx$$
        \end{proof}

        \item If $f$ and $g$ are inverse functions and $f'$ is continuous, prove that $$\int_a^b f(x) dx = bf(b) - af(a) - \int_{f(a)}^{f(b)} g(y) dy$$

        \begin{proof}

            By part (a), we know $$\int_a^b f(x) dx = bf(b) - af(a) - \int_a^b xf'(x) dx$$

            which is equivalent to $$\int_a^b f(x) dx = bf(b) - af(a) - \int_a^b x d f(x)$$

            $\because x = g(f(x))$
            
            $\therefore $ let $y = f(x)$, then 

            $$\int_a^b f(x) dx = bf(b) - af(a) - \int_{f(a)}^{f(b)} g(y) dy$$
        \end{proof}

        \item I just omit the graph.
        \item Use part(b) to evaluate $\int_1^e \ln x dx$

        $$\int_1^e \ln x dx = e - 0 - \int_0^1 e^y dy = e - 0 - (e - 1) = 1$$
    \end{enumerate}
    % 15 17 21 26 30 37 38 70
\end{document}