\documentclass{article}
\usepackage{amsmath}
\usepackage{amsthm}
\usepackage{amssymb}
\usepackage{enumerate}
\usepackage{graphicx}

\newenvironment{solution}{
    \par \textbf{Solution: } \quad \par
}{\par}
% done 
\begin{document}
    \title{Chapter 3 Third Exercise}
    \author{Wang Yue from CS Elite Class}
    \date{\today}

    \maketitle

    \section*{Exercise 3.5}

    \subsection*{27. $x^2 + xy + y^2 = 3, (1,1)$ (ellipse)}

    Take derivative on both sides, and we get $$2x + y + xy' + 2yy' = 0$$

    $$y' = -\frac{2x + y}{x + 2y}$$

    When $x = 1, y = 1$, $y' = -\frac{3}{3} = -1$

    So the slope of the tangent line is $-1$.

    \subsection*{28. $x^2 + 2xy - y^2 + x = 2, (1, 2)$ (hyperbola)}

    Take derivative on both sides, and we get $$2x + 2y + 2xy' - 2yy' + 1 = 0$$

    $$y' = \frac{-1 - 2x - 2y}{2x - 2y}$$

    When $x = 1, y = 2$, $y' = \frac{-1 -2 -4}{-2} = \frac 7 2$

    So the slope of the tangent line is $\frac 7 2$.

    \subsection*{29. $x^2 + y^2 = (2x^2 + 2y^2 - x)^2, (0, \frac 1 2)$, (cardioid)}

    Take derivative on both sides, and we get $$2x + 2yy' = 2(2x^2 + 2y^2 - x)(4x + 4yy' - 1)$$

    $$y' = -\frac{8x^3 - 6x^2 + 8xy^2 - 2y^2}{8x^2y + 8y^3 - 4xy - y}$$

    When $x = 0, y = \frac 1 2, y' = -\frac{-2y^2}{8y^3 - y} = \frac{2y}{8y^2 - 1} = \frac{1}{2 - 1} = 1$

    \subsection*{30. $x^{\frac 2 3} + y^{\frac 2 3} = 4, (-3\sqrt 3, 1)$ (astroid)}

    Taking derivative on both sides, and we get $$\frac 2 3 x^{-\frac 1 3} + \frac 2 3 y^{-\frac 1 3}y' = 0$$

    $$y' = -\frac{x^{-\frac 1 3}}{y^{-\frac 1 3}} = -\sqrt[3]{\frac x y}$$

    When $x = -3\sqrt 3, y = 1, y' = -\sqrt[3]{-3\sqrt 3} = -(-\sqrt 3) = \sqrt 3$
    
    \subsection*{31. $2(x^2 + y^2)^2 = 25(x^2 - y^2), (3, 1)$ (lemniscate)}

    Taking derivative on both sides, and we get $$4(x^2 + y^2)(2x + 2yy') = 25(2x - 2yy')$$

    $$y' = \frac{x[25 - (4x^2 + 4y^2)]}{y[25 + (4x^2 + 4y^2)]}$$

    When $x = 3, y = 1, y' = 3 \frac{25 - 40}{25 + 40} = -\frac{3}{13}$

    \subsection*{32. $y^2(y^2 - 4) = x^2(x^2 - 5), (0, -2)$ (devil's curve)}

    Taking derivative on both sides, and we get $$4y^3y' - 8yy' = 4x^3 - 10x$$

    $$y' = \frac{2x^3 - 5x}{2y^3 - 4y}$$

    When $x = 0, y = -2$, $y' = \frac{0}{-16 + 8} = 0$


    \subsection*{36. $\sqrt x + \sqrt y = 1$}

    Taking derivative on both sides, and we get $$\frac 1 2(x^{-\frac 1 2} + y^{-\frac 1 2}y') = 0$$

    $$y' = -\frac{x^{-\frac 1 2}}{y^{-\frac 1 2}}$$

    $$y'' = -\frac{-\frac 1 2 x^{-\frac 3 2} y^{-\frac 1 2} + x^{-\frac 1 2}\frac 1 2 y^{-\frac 3 2}y'}{(-\frac 1 2y^{-\frac 3 2}) ^2}$$

    $$y'' = 2(x^{-\frac 3 2} y^{\frac 5 2}+x^{-1} y^{2})$$


    \subsection*{51. $y = \sin ^{-1} (2x + 1)$}

    $\because \frac{d \arcsin x}{dx} = \frac{1}{\sqrt{1 - x^2}}$

    $\therefore$ $$y' = 2\frac{1}{\sqrt{- 4x^2 - 4x}} = \frac{1}{\sqrt{-x^2 - x}}$$

    \subsection*{57. $y = x\sin^{-1}x + \sqrt{1 - x^2}$}

    $$y' = x\frac{1}{\sqrt{1 - x^2}} + \arcsin x + \frac 1 2 \frac{1}{\sqrt{1 - x^2}}(-2) = \arcsin x - \frac{\sqrt{1 - x^2}}{x + 1}$$

    \subsection*{60. $y = \arctan \sqrt{\frac {1 - x}{1 + x}}$}

    $$y' = \frac{1}{1 + (\sqrt{\frac{1 - x}{1 + x}})^2} \frac{-1 - x - 1 + x}{(1 + x)^2} = \frac{1 + x}{2} \frac{-2}{(1 + x)^2} = \frac{-1}{1 + x}$$

    \section*{Exercise 3.6}

    \subsection*{16. $y = \ln|1 + t - t^3|$}

    $$y' = \frac{1 - 3t^2}{1 + t - t^3}$$

    \subsection*{18. $y = \ln |\cos (\ln x)|$}

    $$y' = \frac{-\sin \ln x }{x\cos \ln x} = -\frac{\tan \ln x}{x}$$

    \subsection*{25. $y = ln(x + \sqrt{1 + x^2})$}

    $$y' = \frac{1 + \frac{x}{\sqrt{1 + x^2}}}{x + \sqrt{1 + x^2}}$$

    $$\begin{aligned}
        y'' &= \frac{\frac{1}{\sqrt{1 + x^2}} (x + \sqrt{1 + x^2}) - (1 + \frac{x}{\sqrt{1 + x^2}})(1 + \frac{x}{\sqrt{1 + x^2}})}{(x + \sqrt{1 + x^2})^2} \\
        &= \frac{\frac{3x}{\sqrt{1 + x^2}} + x^2 - \frac{x^2}{1 + x^2} }{(x + \sqrt{1 + x^2})^2} \\
        &= \frac{x(3\sqrt{1 + x^2} + 1)}{(1 + x^2)(x + \sqrt{1 + x^2}) ^2}
    \end{aligned}$$

    \subsection*{41. $y = \sqrt{\frac{x - 1}{x^4 + 1}}$}

    $$\ln y = \frac 1 2 \ln \frac{x - 1}{x^4 + 1}$$

    $$\frac{y'}{y} = \frac 1 2 \frac{x^4 + 1}{x - 1} \times \frac{4x^3 + 1}{(x^4 + 1)^2}$$

    $$y' = \frac{4x^3 + 1}{2(x - 1)(x^4 + 1)} \sqrt{\frac{x- 1}{x^4 + 1}} = \frac{4x^3 + 1}{2} \sqrt{\frac{x^4 + 1}{x - 1}}$$

    \subsection*{45. $y = x^{\sin x }$}

    $$\ln y = \ln x^{\sin x} = \sin x \ln x$$

    $$\frac{y'}{y} = \cos x \ln x + \frac{\sin x}{x}$$

    $$y' = x^{\sin x}(\cos x \ln x + \frac{\sin x}{x})$$

    \subsection*{48. $y = (\sin x)^{\ln x}$}

    $$\ln y = \ln (\sin x)^{\ln x} = \ln x \ln \sin x$$

    $$\frac{y'}{y} = \frac{\ln \sin x}{x} + \frac{\cos x \ln x}{\sin x}$$

    $$y' = (\sin x)^{\ln x}(\frac{\ln \sin x}{x} + \frac{\cos x \ln x}{\sin x})$$

    \subsection*{52. Find $y'$ if $x^y = y^x$.}

    Take logarithm on both sides, and we get $$\ln x^y = \ln y^x \iff y\ln x = x\ln y$$

    Taking derivative on both sides, we have $$y'\ln x + \frac{y}{x} = \ln y + x\frac{y'}{y}$$

    $$y' = \frac{\ln y - \frac y x}{\ln x - \frac x y}$$

    \subsection*{53. Find a formula for $f^{(n)} (x)$ if $f(x) = \ln(x - 1)$}

    $\because f'(x) = \frac{1}{x - 1}, f''(x) = \frac{-1}{(x - 1)^2}, f'''(x) = \frac{2}{(x - 1)^3}$

    $\therefore$ we guess that $$f^{(n)} (x) = \frac{(-1)^{n - 1}((n - 1)!}{(x - 1)^n}$$

    We will prove it by mathematical induction.

    When $n = 1$, $f^{(1)}(x) = \frac{1}{x - 1}$, which satisfies the assumption.

    When $n \geq 2$, suppose the assumption holds when $n = k(k \in N_+)$, which means that $$f^{(k)} (x) = \frac{(-1)^{k - 1}(k - 1)!}{(x - 1)^k}$$

    $$
    \begin{aligned}
        f^{(k + 1)}(x) &= \frac{-(-1)^{k - 1}  (k - 1)!\times k(x + 1)^{k - 1}}{(x + 1)^{2k}} \\
        &= \frac{(-1)^k k!}{(x + 1)^{k + 1}}
    \end{aligned}
    $$

    By the proof above, we can conclude that $f^{(n)} x = \frac{(-1)^{n - 1}((n - 1)!}{(x - 1)^n}$

\end{document}
% 3.5: 27 28 29 30 31 32 36 51 57 60
% 3.6: 16 18 25 41 45 48 52 53